src/lib/communication/DY.Lib.Communication.Core.Properties.fst
@@ -25,7 +25,7 @@ open DY.Lib.Communication.Core.Lemmas
 val conf_message_secrecy:
   {|protocol_invariants|} ->
   #a:Type -> {|comm_layer_core_config a|} ->
-  tr:trace -> i:timestamp ->
+  tr:trace ->
   higher_layer_preds:comm_core_higher_layer_event_preds a ->
   receiver:principal ->
   payload:a ->
@@ -33,29 +33,30 @@ val conf_message_secrecy:
   (requires
     trace_invariant tr /\
     has_communication_layer_core_predicates higher_layer_preds /\
-    event_triggered_at tr i receiver (CommConfReceiveMsg receiver payload <: communication_core_event a)
+    event_triggered tr receiver (CommConfReceiveMsg receiver payload <: communication_core_event a)
   )
   (ensures
-    is_well_formed a (is_knowable_by (principal_label receiver) (prefix tr i)) payload /\
-    ((exists sender. higher_layer_preds.send_conf (prefix tr i) sender receiver payload) \/
-    is_well_formed a (is_publishable (prefix tr i)) payload)
+    is_well_formed a (is_knowable_by (principal_label receiver) tr) payload /\
+    ((exists sender. higher_layer_preds.send_conf tr sender receiver payload) \/
+    is_well_formed a (is_publishable tr) payload)
   )
-let conf_message_secrecy #invs #a tr i higher_layer_preds receiver payload =
+let conf_message_secrecy #invs #a tr higher_layer_preds receiver payload =
   let send_event sender:communication_core_event a = CommConfSendMsg sender receiver payload in
+  let i = find_event_triggered_at_timestamp tr receiver (CommConfReceiveMsg receiver payload <: communication_core_event a) in
   let tr_i = prefix tr i in
   eliminate (exists sender. event_triggered tr_i sender (send_event sender)) \/
             is_well_formed a (is_publishable tr_i) payload
   returns
-    is_well_formed a (is_knowable_by (principal_label receiver) tr_i) payload /\
-    ((exists sender. higher_layer_preds.send_conf (prefix tr i) sender receiver payload) \/
-    is_well_formed a (is_publishable (prefix tr i)) payload)
+    is_well_formed a (is_knowable_by (principal_label receiver) tr) payload /\
+    ((exists sender. higher_layer_preds.send_conf tr sender receiver payload) \/
+    is_well_formed a (is_publishable tr) payload)
   with _. eliminate exists sender. event_triggered tr_i sender (send_event sender)
     returns _
     with _. (
       let j = find_event_triggered_at_timestamp tr sender (send_event sender) in
       find_event_triggered_at_timestamp_later tr_i tr sender (send_event sender);
 
-      higher_layer_preds.send_conf_later (prefix tr j) tr_i sender receiver payload;
+      higher_layer_preds.send_conf_later (prefix tr j) tr sender receiver payload;
       ()
     )
   and _. ()
